src/StepSim.v
@@ -1,0 +1,86 @@
+Require Import Oeuf.
+Require Import CompilationUnit.
+Require Import HList.
+Require Import Untyped.
+Require Import StepLib.
+
+Require Import compcert.lib.Coqlib.
+Require Import compcert.ia32.Asm.
+Require Import compcert.common.AST.
+Require Import compcert.common.Smallstep.
+Require Import compcert.common.Errors.
+Require Import compcert.common.Events.
+Require Import compcert.common.Globalenvs.
+
+Require Import UntypedComp.
+
+Require Import StructTact.StructTactics.
+Require Import StructTact.Util.
+
+Require Import EricTact.
+
+
+Section Simulation.
+
+  Variable prog : compilation_unit.
+  Variable tprog : Asm.program.
+  Hypothesis TRANSF : transf_to_asm prog = OK tprog.
+  Definition ge := Genv.globalenv tprog.
+
+(* Dummy top level definition, fill in later *)
+Inductive correspond {tys ty} (exp : SourceLang.expr tys ty) (st : Asm.state).
+
+
+Inductive match_states {tys ty} : SourceLang.expr tys ty -> Asm.state -> Prop :=
+| match_st :
+    forall exp uexp lexp texp E T asm_st,
+      uexp = @UntypedComp.compile tys ty exp ->
+      LiftedComp.match_states E uexp lexp ->
+      TaggedComp.match_states E T lexp texp ->
+      match_states exp asm_st.
+      
+  
+Lemma match_correspond :
+  forall {tys ty} (exp : SourceLang.expr tys ty) st,
+    match_states exp st ->
+    correspond exp st.
+Proof.
+Admitted.
+
+Lemma correspond_initial_match :
+  forall {tys ty} expr,
+      CompilationUnit.initial_state prog tys ty expr ->
+      forall st,
+        Asm.initial_state tprog st ->
+        correspond expr st ->
+        match_states expr st.
+Proof.
+Admitted.
+
+
+Lemma step_sim :
+  forall {tys ty} (exp exp' : SourceLang.expr tys ty),
+    SourceLang.step exp exp' ->
+    forall st,
+      match_states exp st ->
+      exists st',
+        plus Asm.step ge st E0 st' /\
+        match_states exp' st'.
+Proof.
+  intros.
+  replace (@SourceLang.step tys ty) with (@UntypedComp.S.step tys ty) in H by reflexivity.
+  eapply UntypedComp.forward_simulation in H.
+  replace UntypedComp.U.step with LiftedComp.U.step in H by reflexivity.
+  inv H0.
+  eapply LiftedComp.step_sim in H; eauto.
+  break_exists. break_and.
+  eapply TaggedComp.step_sim in H; eauto.
+  break_exists. break_and.
+
+
+  
+
+  
+Admitted.
+
+End Simulation.
